library/init/algebra/ordered_field.lean
@@ -341,13 +341,13 @@ lemma exists_add_lt_and_pos_of_lt {a b : α} (h : b < a) : ∃ c : α, b + c < a
 begin
   apply exists.intro ((a - b) / (1 + 1)),
   split,
-  {assert h2 : a + a > (b + b) + (a - b),
+  {note h2 : a + a > (b + b) + (a - b),
     calc
       a + a > b + a             : add_lt_add_right h _
         ... = b + a + b - b     : by rw add_sub_cancel
         ... = b + b + a - b     : by simp
         ... = (b + b) + (a - b) : by rw add_sub,
-   assert h3 : (a + a) / 2 > ((b + b) + (a - b)) / 2,
+   note h3 : (a + a) / 2 > ((b + b) + (a - b)) / 2,
      exact div_lt_div_of_lt_of_pos h2 two_pos,
    rw [one_add_one_eq_two, sub_eq_add_neg],
    rw [add_self_div_two, -div_add_div_same, add_self_div_two, sub_eq_add_neg] at h3,
